@prefix dc: <http://purl.org/dc/terms/> .
@prefix owl: <http://www.w3.org/2002/07/owl#> .
@prefix rdf: <http://www.w3.org/1999/02/22-rdf-syntax-ns#> .
@prefix rdfs: <http://www.w3.org/2000/01/rdf-schema#> .
@prefix cred: <https://w3.org/2018/credentials#> .
@prefix schema: <http://schema.org/> .
@prefix xsd: <http://www.w3.org/2001/XMLSchema#> .

# CSVM Ontology definition
cred: a owl:Ontology;
  dc:title "Verifiable Claims Vocabulary"@en;
  dc:description """This document describes the RDFS vocabulary description used for Verifiable Claims [[verifiable-claims-data-model]] along with the default JSON-LD Context."""@en;
  dc:date "2018-11-14"^^xsd:date;
  dc:imports <http://purl.org/dc/terms/>, <https://w3.org/2018/security>;
  rdfs:seeAlso <https://www.w3.org/TR/verifiable-claims-data-model/>;

# Class definitions
cred:Policy a rdfs:Class;
  rdfs:label "Policy"@en;
  rdfs:comment """Issue: Generic policy with possible instance 0drlPolicy2017."""@en;
  rdfs:isDefinedBy cred: .
cred:VerifiableCredential a rdfs:Class;
  rdfs:label "Verifiable Credential"@en;
  rdfs:comment """A `verifiable credential` is a credential that is tamper-resistant and whose authorship can be cryptographically verified."""@en;
  rdfs:isDefinedBy cred: .
cred:VerifiablePresentation a rdfs:Class;
  rdfs:label "Verifiable Presentation"@en;
  rdfs:comment """A `verifiable presentation` is a presentation that is made tamper-resistant by the holder."""@en;
  rdfs:isDefinedBy cred: .

# Property definitions
cred:credentialStatus a rdf:Property;
  rdfs:label "credential status"@en;
  rdfs:comment """The value of this property MUST be a status scheme that provides enough information to determine the current status of the credential (e.g. suspended, revoked, etc.). The status scheme will vary depending on a variety of factors, such as whether it is simple to implement or privacy-enhancing."""@en;
  rdfs:domain cred:VerifiableCredential;
  rdfs:isDefinedBy cred: .
cred:credentialSubject a rdf:Property;
  rdfs:label "credentialSubject"@en;
  rdfs:comment """The primary `subject` of a credential."""@en;
  rdfs:domain cred:VerifiableCredential;
  rdfs:isDefinedBy cred: .
cred:evidence a rdf:Property;
  rdfs:label "evidence"@en;
  rdfs:comment """The value of this property MUST be one or more evidence schemes that provides enough information to a verifier to determine whether or not the evidence gathered meets their requirements."""@en;
  rdfs:domain cred:VerifiableCredential;
  rdfs:range cred:DocumentationVerifier;
  rdfs:isDefinedBy cred: .
cred:expirationDate a rdf:Property;
  rdfs:label "expiration date"@en;
  rdfs:comment """The value of this property MUST be a string value of an [[ISO8601]] combined date and time string and represents the date and time the `credential` will cease to be valid"""@en;
  rdfs:domain cred:VerifiableCredential;
  rdfs:range xsd:dateTime;
  rdfs:isDefinedBy cred: .
cred:issuanceDate a rdf:Property;
  rdfs:label "issuance date"@en;
  rdfs:comment """The value of this property MUST be a string value of an [[ISO8601]] combined date and time string and represents the date and time the `credential` was issued. Note that this date represents the earliest date when the information associated with the _claim property became valid."""@en;
  rdfs:domain cred:VerifiableCredential;
  rdfs:range xsd:dateTime;
  rdfs:isDefinedBy cred: .
cred:issuer a rdf:Property;
  rdfs:label "issuer"@en;
  rdfs:comment """The value of this property MUST be a URI. It is RECOMMENDED that dereferencing the URI results in a document containing machine-readable information about the issuer that may be used to verify the information expressed in the `credential`."""@en;
  rdfs:domain cred:VerifiableCredential;
  rdfs:isDefinedBy cred: .
cred:revocation a rdf:Property;
  rdfs:label "revocation"@en;
  rdfs:comment """FIXME"""@en;
  rdfs:domain cred:VerifiableCredential;
  rdfs:isDefinedBy cred: .
cred:termsOfUse a rdf:Property;
  rdfs:label "terms of use"@en;
  rdfs:comment """The value of this property MUST be one or more terms of use descriptions that provide enough information to a verifier to determine how they may utilize the given information."""@en;
  rdfs:domain cred:VerifiableCredential;
  rdfs:range cred:Policy;
  rdfs:isDefinedBy cred: .
cred:verifiableCredential a rdf:Property;
  rdfs:label "verifiable credential"@en;
  rdfs:comment """The contents of the `verifiableCredential` property are `verifiable credentials` as described by this specification."""@en;
  rdfs:domain cred:VerifiablePresentation;
  rdfs:range cred:Credential;
  rdfs:isDefinedBy cred: .
