{
  "@context": [
    {
      "@version": 1.1
    },
    "https://w3.org/2018/security/v1",
    {
      "id": "@id",
      "type": "@type",
      "cred": "https://w3.org/2018/credentials#",
      "dc": "http://purl.org/dc/terms/",
      "schema": "http://schema.org/",
      "xsd": "http://www.w3.org/2001/XMLSchema#",
      "created": {
        "@id": "dc:created",
        "@type": "xsd:dateTime"
      },
      "creator": {
        "@id": "dc:creator",
        "@type": "@id"
      },
      "Policy": "cred:Policy",
      "VerifiableCredential": "cred:VerifiableCredential",
      "VerifiablePresentation": "cred:VerifiablePresentation",
      "claim": {
        "@id": "cred:claim",
        "@container": "@graph",
        "@type": "@id"
      },
      "credentialStatus": {
        "@id": "cred:credentialStatus",
        "@type": "@id"
      },
      "evidence": {
        "@id": "cred:evidence",
        "@type": "@id"
      },
      "expirationDate": {
        "@id": "cred:expirationDate",
        "@type": "xsd:dateTime"
      },
      "issuanceDate": {
        "@id": "cred:issuanceDate",
        "@type": "xsd:dateTime"
      },
      "issuer": {
        "@id": "cred:issuer",
        "@type": "@id"
      },
      "revocation": {
        "@id": "cred:revocation",
        "@type": "@id"
      },
      "termsOfUse": {
        "@id": "cred:termsOfUse",
        "@type": "@id"
      },
      "verifiableCredential": {
        "@id": "cred:verifiableCredential",
        "@type": "@id",
        "@container": "@graph"
      }
    }
  ],
  "@graph": {
    "@context": {
      "id": "@id",
      "type": "@type",
      "dc": "http://purl.org/dc/terms/",
      "owl": "http://www.w3.org/2002/07/owl#",
      "rdf": "http://www.w3.org/1999/02/22-rdf-syntax-ns#",
      "rdfs": "http://www.w3.org/2000/01/rdf-schema#",
      "dc:title": {
        "@container": "@language"
      },
      "dc:description": {
        "@container": "@language"
      },
      "dc:date": {
        "@type": "xsd:date"
      },
      "rdfs:comment": {
        "@container": "@language"
      },
      "rdfs:domain": {
        "@type": "@id"
      },
      "rdfs:label": {
        "@container": "@language"
      },
      "rdfs:range": {
        "@type": "@id"
      },
      "rdfs:seeAlso": {
        "@type": "@id"
      },
      "rdfs:subClassOf": {
        "@type": "@id"
      },
      "rdfs:subPropertyOf": {
        "@type": "@id"
      },
      "owl:equivalentClass": {
        "@type": "@vocab"
      },
      "owl:equivalentProperty": {
        "@type": "@vocab"
      },
      "owl:oneOf": {
        "@container": "@list",
        "@type": "@vocab"
      },
      "owl:imports": {
        "@type": "@id"
      },
      "owl:versionInfo": {
        "@type": "@id"
      },
      "owl:inverseOf": {
        "@type": "@vocab"
      },
      "owl:unionOf": {
        "@type": "@vocab",
        "@container": "@list"
      },
      "rdfs_classes": {
        "@reverse": "rdfs:isDefinedBy",
        "@type": "@id"
      },
      "rdfs_properties": {
        "@reverse": "rdfs:isDefinedBy",
        "@type": "@id"
      },
      "rdfs_datatypes": {
        "@reverse": "rdfs:isDefinedBy",
        "@type": "@id"
      },
      "rdfs_instances": {
        "@reverse": "rdfs:isDefinedBy",
        "@type": "@id"
      }
    },
    "@id": "https://w3.org/2018/credentials#",
    "@type": "owl:Ontology",
    "dc:title": {
      "en": "Verifiable Claims Vocabulary"
    },
    "dc:description": {
      "en": "This document describes the RDFS vocabulary description used for Verifiable Claims [[verifiable-claims-data-model]] along with the default JSON-LD Context."
    },
    "dc:date": "2018-07-25",
    "owl:imports": [
      "http://purl.org/dc/terms/",
      "https://w3.org/2018/security"
    ],
    "rdfs:seeAlso": [
      "https://www.w3.org/TR/verifiable-claims-data-model/"
    ],
    "rdfs_classes": [
      {
        "@id": "cred:Policy",
        "@type": "rdfs:Class",
        "rdfs:label": {
          "en": "Policy"
        },
        "rdfs:comment": {
          "en": "Issue: Generic policy with possible instance 0drlPolicy2017."
        }
      },
      {
        "@id": "cred:VerifiableCredential",
        "@type": "rdfs:Class",
        "rdfs:label": {
          "en": "Verifiable Credential"
        },
        "rdfs:comment": {
          "en": "A `verifiable credential` is a credential that is tamper-resistant and whose authorship can be cryptographically verified."
        }
      },
      {
        "@id": "cred:VerifiablePresentation",
        "@type": "rdfs:Class",
        "rdfs:label": {
          "en": "Verifiable Presentation"
        },
        "rdfs:comment": {
          "en": "A `verifiable presentation` is a presentation that is made tamper-resistant by the holder."
        }
      }
    ],
    "rdfs_properties": [
      {
        "@id": "cred:claim",
        "@type": "rdf:Property",
        "rdfs:label": {
          "en": "claim"
        },
        "rdfs:comment": {
          "en": "A statement made about a `subject`."
        },
        "rdfs:domain": "cred:VerifiableCredential"
      },
      {
        "@id": "cred:credentialStatus",
        "@type": "rdf:Property",
        "rdfs:label": {
          "en": "credential status"
        },
        "rdfs:comment": {
          "en": "The value of this property MUST be a status scheme that provides enough information to determine the current status of the credential (e.g. suspended, revoked, etc.). The status scheme will vary depending on a variety of factors, such as whether it is simple to implement or privacy-enhancing."
        },
        "rdfs:domain": "cred:VerifiableCredential"
      },
      {
        "@id": "cred:evidence",
        "@type": "rdf:Property",
        "rdfs:label": {
          "en": "evidence"
        },
        "rdfs:comment": {
          "en": "The value of this property MUST be one or more evidence schemes that provides enough information to a verifier to determine whether or not the evidence gathered meets their requirements."
        },
        "rdfs:domain": "cred:VerifiableCredential",
        "rdfs:range": "cred:DocumentationVerifier"
      },
      {
        "@id": "cred:expirationDate",
        "@type": "rdf:Property",
        "rdfs:label": {
          "en": "expiration date"
        },
        "rdfs:comment": {
          "en": "The value of this property MUST be a string value of an [[ISO8601]] combined date and time string and represents the date and time the `credential` will cease to be valid"
        },
        "rdfs:domain": "cred:VerifiableCredential",
        "rdfs:range": "xsd:dateTime"
      },
      {
        "@id": "cred:issuanceDate",
        "@type": "rdf:Property",
        "rdfs:label": {
          "en": "issuance date"
        },
        "rdfs:comment": {
          "en": "The value of this property MUST be a string value of an [[ISO8601]] combined date and time string and represents the date and time the `credential` was issued. Note that this date represents the earliest date when the information associated with the _claim property became valid."
        },
        "rdfs:domain": "cred:VerifiableCredential",
        "rdfs:range": "xsd:dateTime"
      },
      {
        "@id": "cred:issuer",
        "@type": "rdf:Property",
        "rdfs:label": {
          "en": "issuer"
        },
        "rdfs:comment": {
          "en": "The value of this property MUST be a URI. It is RECOMMENDED that dereferencing the URI results in a document containing machine-readable information about the issuer that may be used to verify the information expressed in the `credential`."
        },
        "rdfs:domain": "cred:VerifiableCredential"
      },
      {
        "@id": "cred:revocation",
        "@type": "rdf:Property",
        "rdfs:label": {
          "en": "revocation"
        },
        "rdfs:comment": {
          "en": "FIXME"
        },
        "rdfs:domain": "cred:VerifiableCredential"
      },
      {
        "@id": "cred:termsOfUse",
        "@type": "rdf:Property",
        "rdfs:label": {
          "en": "terms of use"
        },
        "rdfs:comment": {
          "en": "The value of this property MUST be one or more terms of use descriptions that provide enough information to a verifier to determine how they may utilize the given information."
        },
        "rdfs:domain": "cred:VerifiableCredential",
        "rdfs:range": "cred:Policy"
      },
      {
        "@id": "cred:verifiableCredential",
        "@type": "rdf:Property",
        "rdfs:label": {
          "en": "verifiable credential"
        },
        "rdfs:comment": {
          "en": "The contents of the `verifiableCredential` property are `verifiable credentials` as described by this specification."
        },
        "rdfs:domain": "cred:VerifiablePresentation",
        "rdfs:range": "cred:Credential"
      }
    ]
  }
}
