@prefix dc: <http://purl.org/dc/terms/> .
@prefix owl: <http://www.w3.org/2002/07/owl#> .
@prefix rdf: <http://www.w3.org/1999/02/22-rdf-syntax-ns#> .
@prefix rdfs: <http://www.w3.org/2000/01/rdf-schema#> .
@prefix cred: <https://w3id.org/credentials#> .
@prefix schema: <http://schema.org/> .
@prefix sec: <https://w3id.org/security#> .
@prefix xsd: <http://www.w3.org/2001/XMLSchema#> .

# CSVM Ontology definition
cred: a owl:Ontology;
  dc:title "Verifiable Claims Vocabulary"@en;
  dc:description """This document describes the RDFS vocabulary description used for Verifiable Claims [[verifiable-claims-data-model]] along with the default JSON-LD Context."""@en;
  dc:date "2017-12-01"^^xsd:date;
  dc:imports <http://purl.org/dc/terms/>, <https://w3id.org/security>;
  rdfs:seeAlso <https://www.w3.org/TR/verifiable-claims-data-model/>;

# Class definitions
cred:Credential a rdfs:Class;
  rdfs:label "Credential"@en;
  rdfs:comment """FIXME"""@en;
  rdfs:isDefinedBy cred: .
cred:CryptographicKeyCredential a rdfs:Class;
  rdfs:label "Cryptographic Key Credential"@en;
  rdfs:comment """FIXME"""@en;
  rdfs:subClassOf cred:Credential;
  rdfs:isDefinedBy cred: .
cred:Profile a rdfs:Class;
  rdfs:label "Verifiable Profile"@en;
  rdfs:comment """A set of one or more `credentials` typically related to the same `subject`. An entity may have multiple `profiles` and each `profile` may contain `verifiable credentials` issued by multiple issuers. A `verifiable profile` is a `profile` that is tamper-resistant and whose contents are typically counter-signed by the `holder` or `subject`."""@en;
  rdfs:isDefinedBy cred: .
cred:RevocationList2017 a rdfs:Class;
  rdfs:label "Revocation List 2017"@en;
  rdfs:comment """FIXME"""@en;
  rdfs:subClassOf cred:RevocationList2017;
  rdfs:isDefinedBy cred: .

# Property definitions
cred:claim a rdf:Property;
  rdfs:label "claim"@en;
  rdfs:comment """A statement made about a `subject`. A **verifiable claim** is a claim that is tamper-resistant and whose authorship can be cryptographically verified."""@en;
  rdfs:domain cred:Credential;
  rdfs:isDefinedBy cred: .
cred:credential a rdf:Property;
  rdfs:label "credential"@en;
  rdfs:comment """A set of one or more claims made by the same `entity` about a `subject`. A **verifiable credential** is a credential that is tamper-resistant and whose authorship can be cryptographically verified."""@en;
  rdfs:domain cred:Profile;
  rdfs:range cred:Credential;
  rdfs:isDefinedBy cred: .
cred:evidence a rdf:Property;
  rdfs:label "evidence"@en;
  rdfs:comment """The value of this property MUST be one or more evidence schemes that provides enough information to a verifier to determine whether or not the evidence gathered meets their requirements."""@en;
  rdfs:domain cred:Credential;
  rdfs:range cred:DocumentationVerifier;
  rdfs:isDefinedBy cred: .
cred:issued a rdf:Property;
  rdfs:label "issued"@en;
  rdfs:comment """The value of this property MUST be a string value of an [[ISO8601]] combined date and time string and represents the date and time the `credential` was issued. Note that this date represents the earliest date when the information associated with the _claim property became valid."""@en;
  rdfs:domain cred:Credential;
  rdfs:range xsd:dateTime;
  rdfs:isDefinedBy cred: .
cred:issuer a rdf:Property;
  rdfs:label "issuer"@en;
  rdfs:comment """An `entit`y that creates a `verifiable claim`, associates it with a particular `subject`, and transmits it to a `holder`."""@en;
  rdfs:domain cred:Credential;
  rdfs:isDefinedBy cred: .
cred:recipient a rdf:Property;
  rdfs:label "recipient"@en;
  rdfs:comment """FIXME"""@en;
  rdfs:isDefinedBy cred: .
cred:referenceId a rdf:Property;
  rdfs:label "referenceId"@en;
  rdfs:comment """FIXME"""@en;
  rdfs:isDefinedBy cred: .
cred:revocation a rdf:Property;
  rdfs:label "revocation"@en;
  rdfs:comment """"""@en;
  rdfs:domain cred:Credential;
  rdfs:range cred:RevocationList2017;
  rdfs:isDefinedBy cred: .
