{
  "@context": {
    "id": "@id",
    "type": "@type",
    "cred": "https://w3id.org/credentials#",
    "dc": "http://purl.org/dc/terms/",
    "schema": "http://schema.org/",
    "sec": "https://w3id.org/security#",
    "xsd": "http://www.w3.org/2001/XMLSchema#",
    "CryptographicKey": "sec:Key",
    "GraphSignature2012": "sec:GraphSignature2012",
    "Identity": "https://w3id.org/identity#Identity",
    "LinkedDataSignature2015": "sec:LinkedDataSignature2015",
    "created": {
      "@id": "dc:created",
      "@type": "xsd:dateTime"
    },
    "creator": {
      "@id": "dc:creator",
      "@type": "@id"
    },
    "domain": "sec:domain",
    "expires": {
      "@id": "sec:expiration",
      "@type": "xsd:dateTime"
    },
    "nonce": "sec:nonce",
    "normalizationAlgorithm": "sec:normalizationAlgorithm",
    "owner": {
      "@id": "sec:owner",
      "@type": "@id"
    },
    "privateKey": {
      "@id": "sec:privateKey",
      "@type": "@id"
    },
    "privateKeyPem": "sec:privateKeyPem",
    "publicKey": {
      "@id": "sec:publicKey",
      "@type": "@id"
    },
    "publicKeyPem": "sec:publicKeyPem",
    "publicKeyService": {
      "@id": "sec:publicKeyService",
      "@type": "@id"
    },
    "revoked": {
      "@id": "sec:revoked",
      "@type": "xsd:dateTime"
    },
    "signature": "sec:signature",
    "signatureAlgorithm": "sec:signatureAlgorithm",
    "signatureValue": "sec:signatureValue",
    "Credential": "cred:Credential",
    "CryptographicKeyCredential": "cred:CryptographicKeyCredential",
    "Profile": "cred:Profile",
    "RevocationList2017": "cred:RevocationList2017",
    "claim": {
      "@id": "cred:claim",
      "@container": "@graph"
    },
    "credential": {
      "@id": "cred:credential",
      "@type": "@id"
    },
    "evidence": {
      "@id": "cred:evidence",
      "@type": "@id"
    },
    "issued": {
      "@id": "cred:issued",
      "@type": "xsd:dateTime"
    },
    "issuer": {
      "@id": "cred:issuer",
      "@type": "@id"
    },
    "recipient": {
      "@id": "cred:recipient",
      "@type": "@id"
    },
    "referenceId": {
      "@id": "cred:referenceId"
    },
    "revocation": "cred:revocation"
  },
  "@graph": {
    "@context": {
      "id": "@id",
      "type": "@type",
      "dc": "http://purl.org/dc/terms/",
      "owl": "http://www.w3.org/2002/07/owl#",
      "rdf": "http://www.w3.org/1999/02/22-rdf-syntax-ns#",
      "rdfs": "http://www.w3.org/2000/01/rdf-schema#",
      "dc:title": {
        "@container": "@language"
      },
      "dc:description": {
        "@container": "@language"
      },
      "dc:date": {
        "@type": "xsd:date"
      },
      "rdfs:comment": {
        "@container": "@language"
      },
      "rdfs:domain": {
        "@type": "@id"
      },
      "rdfs:label": {
        "@container": "@language"
      },
      "rdfs:range": {
        "@type": "@id"
      },
      "rdfs:seeAlso": {
        "@type": "@id"
      },
      "rdfs:subClassOf": {
        "@type": "@id"
      },
      "rdfs:subPropertyOf": {
        "@type": "@id"
      },
      "owl:equivalentClass": {
        "@type": "@vocab"
      },
      "owl:equivalentProperty": {
        "@type": "@vocab"
      },
      "owl:oneOf": {
        "@container": "@list",
        "@type": "@vocab"
      },
      "owl:imports": {
        "@type": "@id"
      },
      "owl:versionInfo": {
        "@type": "@id"
      },
      "owl:inverseOf": {
        "@type": "@vocab"
      },
      "owl:unionOf": {
        "@type": "@vocab",
        "@container": "@list"
      },
      "rdfs_classes": {
        "@reverse": "rdfs:isDefinedBy",
        "@type": "@id"
      },
      "rdfs_properties": {
        "@reverse": "rdfs:isDefinedBy",
        "@type": "@id"
      },
      "rdfs_datatypes": {
        "@reverse": "rdfs:isDefinedBy",
        "@type": "@id"
      },
      "rdfs_instances": {
        "@reverse": "rdfs:isDefinedBy",
        "@type": "@id"
      }
    },
    "@id": "https://w3id.org/credentials#",
    "@type": "owl:Ontology",
    "dc:title": {
      "en": "Verifiable Claims Vocabulary"
    },
    "dc:description": {
      "en": "This document describes the RDFS vocabulary description used for Verifiable Claims [[verifiable-claims-data-model]] along with the default JSON-LD Context."
    },
    "dc:date": "2017-11-16",
    "owl:imports": [
      "http://purl.org/dc/terms/",
      "https://w3id.org/security"
    ],
    "rdfs:seeAlso": [
      "https://www.w3.org/TR/verifiable-claims-data-model/"
    ],
    "rdfs_classes": [
      {
        "@id": "cred:Credential",
        "@type": "rdfs:Class",
        "rdfs:label": {
          "en": "Credential"
        },
        "rdfs:comment": {
          "en": "FIXME"
        }
      },
      {
        "@id": "cred:CryptographicKeyCredential",
        "@type": "rdfs:Class",
        "rdfs:label": {
          "en": "Cryptographic Key Credential"
        },
        "rdfs:comment": {
          "en": "FIXME"
        },
        "rdfs:subClassOf": "cred:Credential"
      },
      {
        "@id": "cred:Profile",
        "@type": "rdfs:Class",
        "rdfs:label": {
          "en": "Verifiable Profile"
        },
        "rdfs:comment": {
          "en": "A set of one or more `credentials` typically related to the same `subject`. An entity may have multiple `profiles` and each `profile` may contain `verifiable credentials` issued by multiple issuers. A `verifiable profile` is a `profile` that is tamper-resistant and whose contents are typically counter-signed by the `holder` or `subject`."
        }
      },
      {
        "@id": "cred:RevocationList2017",
        "@type": "rdfs:Class",
        "rdfs:label": {
          "en": "Revocation List 2017"
        },
        "rdfs:comment": {
          "en": "FIXME"
        },
        "rdfs:subClassOf": "cred:RevocationList2017"
      }
    ],
    "rdfs_properties": [
      {
        "@id": "cred:claim",
        "@type": "rdf:Property",
        "rdfs:label": {
          "en": "claim"
        },
        "rdfs:comment": {
          "en": "A statement made about a `subject`. A **verifiable claim** is a claim that is tamper-resistant and whose authorship can be cryptographically verified."
        },
        "rdfs:domain": "cred:Credential"
      },
      {
        "@id": "cred:credential",
        "@type": "rdf:Property",
        "rdfs:label": {
          "en": "credential"
        },
        "rdfs:comment": {
          "en": "A set of one or more claims made by the same `entity` about a `subject`. A **verifiable credential** is a credential that is tamper-resistant and whose authorship can be cryptographically verified."
        },
        "rdfs:domain": "cred:Profile",
        "rdfs:range": "cred:Credential"
      },
      {
        "@id": "cred:evidence",
        "@type": "rdf:Property",
        "rdfs:label": {
          "en": "evidence"
        },
        "rdfs:comment": {
          "en": "The value of this property MUST be one or more evidence schemes that provides enough information to a verifier to determine whether or not the evidence gathered meets their requirements."
        },
        "rdfs:domain": "cred:Credential",
        "rdfs:range": "cred:DocumentationVerifier"
      },
      {
        "@id": "cred:issued",
        "@type": "rdf:Property",
        "rdfs:label": {
          "en": "issued"
        },
        "rdfs:comment": {
          "en": "The value of this property MUST be a string value of an [[ISO8601]] combined date and time string and represents the date and time the `credential` was issued. Note that this date represents the earliest date when the information associated with the _claim property became valid."
        },
        "rdfs:domain": "cred:Credential",
        "rdfs:range": "xsd:dateTime"
      },
      {
        "@id": "cred:issuer",
        "@type": "rdf:Property",
        "rdfs:label": {
          "en": "issuer"
        },
        "rdfs:comment": {
          "en": "An `entit`y that creates a `verifiable claim`, associates it with a particular `subject`, and transmits it to a `holder`."
        },
        "rdfs:domain": "cred:Credential"
      },
      {
        "@id": "cred:recipient",
        "@type": "rdf:Property",
        "rdfs:label": {
          "en": "recipient"
        },
        "rdfs:comment": {
          "en": "FIXME"
        }
      },
      {
        "@id": "cred:referenceId",
        "@type": "rdf:Property",
        "rdfs:label": {
          "en": "referenceId"
        },
        "rdfs:comment": {
          "en": "FIXME"
        }
      }
    ],
    "rdfs_instances": [
      {
        "@id": "cred:revocation",
        "@type": "rdf:PRoperty",
        "rdfs:label": {
          "en": "revocation"
        },
        "rdfs:comment": {
          "en": ""
        }
      }
    ]
  }
}
